context-defthms.lisp
@@ -1,0 +1,6 @@
+(in-package "ACL2")
+
+(include-book "context")
+
+(defthm mk-dummy-context-validp
+  (context/validp (mk-dummy-context)))
