env-defthms.lisp
@@ -1,3 +1,11 @@
 (in-package "ACL2")
 
 (include-book "stack-defthms")
+
+(defthm mk-env-op-validp
+    (env/validp (mk-env-op anything)))
+
+(defthm env/setsubstate-io-validp
+    (implies (and (env/validp e)
+                  (substate/validp ss))
+             (env/validp (env/set-substate e ss))))
