exec-defthms.lisp
@@ -1,24 +1,27 @@
 (in-package "ACL2")
 
+(include-book "std/lists/top" :dir :system)
+
 (include-book "env")
 (include-book "env-defthms")
 (include-book "exec")
 
-;; (defthm env/exec-step-valid-io-pc
-;;     (implies (env/validp e)
-;;              (integerp (env/pc (env/step e)))))
+(defthm env/step-io-pc-validp
+    (implies (env/validp e)
+             (integerp (env/pc (env/step e)))))
 
-;; (defthm env/exec-hacky-valid-io-pc-limit-step
-;;     (implies (env/validp e)
-;;              (integerp (env/pc (env/exec-hacky e 1)))))
+;; The proof checking takes about 10 minutes.
+(defthm env/step-io-validp
+    (implies (env/validp e)
+             (env/validp (env/step e))))
 
-;; (defthm env/exec-hacky-valid-io-pc
-;;     (implies (env/validp e)
-;;              (integerp (env/pc (env/exec-hacky e n)))))
+(defthm env/exec-hacky-io-pc-validp
+    (implies (env/validp e)
+             (integerp (env/pc (env/exec-hacky e n)))))
 
-;; (defthm env/exec-hacky-valid-io
-;;     (implies (env/validp e)
-;;              (env/validp (env/exec-hacky e n))))
+(defthm env/exec-hacky-io-validp
+    (implies (env/validp e)
+             (env/validp (env/exec-hacky e n))))
 
 ;; (defthm env/exec-valid-io
 ;;     (implies (env/validp e)
