op-exec-defthms.lisp
@@ -1,0 +1,19 @@
+(in-package "ACL2")
+
+(include-book "std/lists/top" :dir :system)
+
+(include-book "env")
+(include-book "env-defthms")
+(include-book "op-exec")
+
+(defthm exec-stop-io-validp
+    (implies (env/validp e)
+             (env/validp (exec-stop e))))
+
+(defthm exec-revert-io-validp
+    (implies (env/validp e)
+             (env/validp (exec-revert e))))
+
+(defthm exec-calldataload-io-validp
+    (implies (env/validp e)
+             (env/validp (exec-calldataload e))))
