substate-defthms.lisp
@@ -1,0 +1,6 @@
+(in-package "ACL2")
+
+(include-book "substate")
+
+(defthm mk-empty-substate-validp
+  (substate/validp (mk-empty-substate)))
